case_study/RiscvPmp/IrisModelBinary.v
@@ -33,7 +33,8 @@ From Katamaran Require Import
      Iris.Model
      Iris.BinaryInstance
      RiscvPmp.Machine
-     RiscvPmp.IrisModel.
+     RiscvPmp.IrisModel
+     RiscvPmp.IrisInstance.
 From iris Require Import
      base_logic.lib.gen_heap
      proofmode.tactics.
@@ -48,6 +49,7 @@ Import RiscvPmpProgram.
 Module RiscvPmpIrisBase2 <: IrisBase2 RiscvPmpBase RiscvPmpProgram RiscvPmpSemantics.
   (* Pull in the definition of the LanguageMixin and register ghost state. *)
   Include RiscvPmpIrisBase.
+  Import RiscvPmpIrisAdeqParameters.
 
   (* Defines the memory ghost state. *)
   Section RiscvPmpIrisParams2.
@@ -62,86 +64,13 @@ Module RiscvPmpIrisBase2 <: IrisBase2 RiscvPmpBase RiscvPmpProgram RiscvPmpSeman
         ; mc_gtGS2_right : traceG Trace Σ
         }.
 
-    Definition memGpreS2 : gFunctors -> Set := fun Σ => prod (RiscvPmpIrisBase.memGpreS Σ) (RiscvPmpIrisBase.memGpreS Σ).
     Definition memGS2 : gFunctors -> Set := mcMemGS2.
-    Definition memΣ2 : gFunctors := gFunctors.app (RiscvPmpIrisBase.memΣ) (RiscvPmpIrisBase.memΣ).
-
-    Definition memΣ_GpreS2 : forall {Σ}, subG memΣ2 Σ -> memGpreS2 Σ :=
-      fun {Σ} HsG => (memΣ_GpreS (Σ := Σ) (fst (subG_inv _ _ _ HsG)),
-                    memΣ_GpreS (Σ := Σ) (snd (subG_inv _ _ _ HsG))).
-
     Definition mem_inv2 : forall {Σ}, mcMemGS2 Σ -> Memory -> Memory -> iProp Σ :=
       fun {Σ} hG μ1 μ2 =>
         (RiscvPmpIrisBase.mem_inv mc_ghGS2_left μ1 ∗ RiscvPmpIrisBase.mem_inv mc_ghGS2_right μ2)%I.
-
-    Definition mem_res2 `{hG : mcMemGS2 Σ} : Memory -> Memory -> iProp Σ :=
-      fun μ1 μ2 => (RiscvPmpIrisBase.mem_res (hG := mc_ghGS2_left) μ1 ∗
-                   RiscvPmpIrisBase.mem_res (hG := mc_ghGS2_right) μ2)%I.
-
-    Lemma mem_inv_init2 `{gHP : prod (RiscvPmpIrisBase.memGpreS Σ) (RiscvPmpIrisBase.memGpreS Σ)} (μ1 μ2 : Memory) :
-      ⊢ |==> ∃ mG : mcMemGS2 Σ, (mem_inv2 mG μ1 μ2 ∗ mem_res2 μ1 μ2)%I.
-    Proof.
-      iMod (RiscvPmpIrisBase.mem_inv_init (gHP := fst gHP) μ1) as (mG1) "[inv1 res1]".
-      iMod (RiscvPmpIrisBase.mem_inv_init (gHP := snd gHP) μ2) as (mG2) "[inv2 res2]".
-      iMod (trace_alloc (memory_trace μ1)) as (gT1) "[Hauth1 Hfrag1]".
-      iMod (trace_alloc (memory_trace μ2)) as (gT2) "[Hauth2 Hfrag2]".
-      iModIntro.
-      iExists (McMemGS2 mG1 mG2 gT1 gT2).
-      iSplitL "inv1 inv2"; iFrame.
-    Qed.
-
-    (* Note: this defaultRegStore is only needed for technical reason, it is not used. *)
-    Definition defaultRegStore : RegStore :=
-      fun τ r =>
-        match r with
-          pc => (bv.zero : TypeDecl.ty.Val ty_xlenbits)
-        | nextpc => (bv.zero : TypeDecl.ty.Val ty_xlenbits)
-        | mstatus => (MkMstatus Machine : TypeDecl.ty.Val ty_mstatus)
-        | mtvec => (bv.zero : TypeDecl.ty.Val ty_xlenbits)
-        | mcause => (bv.zero : TypeDecl.ty.Val ty_xlenbits)
-        | mepc => (bv.zero : TypeDecl.ty.Val ty_xlenbits)
-        | cur_privilege => Machine
-        | x1  => (bv.zero : TypeDecl.ty.Val ty_xlenbits)
-        | x2  => (bv.zero : TypeDecl.ty.Val ty_xlenbits)
-        | x3  => (bv.zero : TypeDecl.ty.Val ty_xlenbits)
-        | x4  => (bv.zero : TypeDecl.ty.Val ty_xlenbits)
-        | x5  => (bv.zero : TypeDecl.ty.Val ty_xlenbits)
-        | x6  => (bv.zero : TypeDecl.ty.Val ty_xlenbits)
-        | x7  => (bv.zero : TypeDecl.ty.Val ty_xlenbits)
-        | x8  => (bv.zero : TypeDecl.ty.Val ty_xlenbits)
-        | x9  => (bv.zero : TypeDecl.ty.Val ty_xlenbits)
-        | x10 => (bv.zero : TypeDecl.ty.Val ty_xlenbits)
-        | x11 => (bv.zero : TypeDecl.ty.Val ty_xlenbits)
-        | x12 => (bv.zero : TypeDecl.ty.Val ty_xlenbits)
-        | x13 => (bv.zero : TypeDecl.ty.Val ty_xlenbits)
-        | x14 => (bv.zero : TypeDecl.ty.Val ty_xlenbits)
-        | x15 => (bv.zero : TypeDecl.ty.Val ty_xlenbits)
-        | x16 => (bv.zero : TypeDecl.ty.Val ty_xlenbits)
-        | x17 => (bv.zero : TypeDecl.ty.Val ty_xlenbits)
-        | x18 => (bv.zero : TypeDecl.ty.Val ty_xlenbits)
-        | x19 => (bv.zero : TypeDecl.ty.Val ty_xlenbits)
-        | x20 => (bv.zero : TypeDecl.ty.Val ty_xlenbits)
-        | x21 => (bv.zero : TypeDecl.ty.Val ty_xlenbits)
-        | x22 => (bv.zero : TypeDecl.ty.Val ty_xlenbits)
-        | x23 => (bv.zero : TypeDecl.ty.Val ty_xlenbits)
-        | x24 => (bv.zero : TypeDecl.ty.Val ty_xlenbits)
-        | x25 => (bv.zero : TypeDecl.ty.Val ty_xlenbits)
-        | x26 => (bv.zero : TypeDecl.ty.Val ty_xlenbits)
-        | x27 => (bv.zero : TypeDecl.ty.Val ty_xlenbits)
-        | x28 => (bv.zero : TypeDecl.ty.Val ty_xlenbits)
-        | x29 => (bv.zero : TypeDecl.ty.Val ty_xlenbits)
-        | x30 => (bv.zero : TypeDecl.ty.Val ty_xlenbits)
-        | x31 => (bv.zero : TypeDecl.ty.Val ty_xlenbits)
-        | pmp0cfg => (MkPmpcfg_ent false OFF true true true : TypeDecl.ty.Val ty_pmpcfg_ent)
-        | pmp1cfg => (MkPmpcfg_ent false OFF true true true : TypeDecl.ty.Val ty_pmpcfg_ent)
-        | pmpaddr0 => (bv.zero : TypeDecl.ty.Val ty_xlenbits)
-        | pmpaddr1 => (bv.zero : TypeDecl.ty.Val ty_xlenbits)
-        end.
-
-    (* Note: this defaultMemory is only needed for technical reason, it is not used. *)
-    Definition defaultMemory : Memory := mkMem (fun a => bv.zero) [] state_init.
   End RiscvPmpIrisParams2.
 
   Include IrisResources2 RiscvPmpBase RiscvPmpProgram RiscvPmpSemantics.
 
 End RiscvPmpIrisBase2.
+
