test/SumMaxLen.v
@@ -346,26 +346,33 @@ Module Import ExampleModel.
 
     Include IrisPrelims DefaultBase ExampleProgram ExampleSemantics.
 
-    Definition memGpreS : gFunctors -> Set := fun Σ => True.
     Definition memGS : gFunctors -> Set := fun Σ => True.
-    Definition memΣ : gFunctors := gFunctors.nil.
-    Definition memΣ_GpreS : forall {Σ}, subG memΣ Σ -> memGpreS Σ := fun _ _ => I.
     Definition mem_inv : forall {Σ}, memGS Σ -> Memory -> iProp Σ := fun Σ mG μ => True%I.
-    Definition mem_res : forall {Σ}, memGS Σ -> Memory -> iProp Σ := fun Σ mG μ => True%I.
-    Lemma mem_inv_init `{gHP : memGpreS Σ} (μ : Memory) :
-      ⊢ |==> ∃ mG : memGS Σ, (mem_inv mG μ ∗ mem_res mG μ)%I.
-    Proof. now iStartProof. Qed.
 
     (* Combine the memory and register ghost states. *)
     Include IrisResources DefaultBase ExampleProgram ExampleSemantics.
 
   End ExampleIrisBase.
 
+  Module ExampleIrisAdeqParams <: IrisAdeqParameters DefaultBase ExampleIrisBase.
+    Import iris.base_logic.lib.gen_heap.
+    Import iris.proofmode.tactics.
+
+    Definition memGpreS : gFunctors -> Set := fun Σ => True.
+    Definition memΣ : gFunctors := gFunctors.nil.
+    Definition memΣ_GpreS : forall {Σ}, subG memΣ Σ -> memGpreS Σ := fun _ _ => I.
+    Definition mem_res : forall {Σ}, memGS Σ -> Memory -> iProp Σ := fun Σ mG μ => True%I.
+    Lemma mem_inv_init `{gHP : memGpreS Σ} (μ : Memory) :
+      ⊢ |==> ∃ mG : memGS Σ, (mem_inv mG μ ∗ mem_res mG μ)%I.
+    Proof. now iStartProof. Qed.
+  End ExampleIrisAdeqParams.
+
+
   (* Finally, include the constructed operational model, the axiomatic program
      logic, and the Iris implementation of the axioms. *)
   Module Import ExampleIrisInstance <:
     IrisInstance DefaultBase ExampleSig ExampleProgram ExampleSemantics
-      ExampleIrisBase.
+      ExampleIrisBase ExampleIrisAdeqParams.
 
     (* There are no user-defined spatial predicates, also use trivial definitions
        here. *)
@@ -381,10 +388,10 @@ Module Import ExampleModel.
     Include IrisSignatureRules DefaultBase ExampleSig ExampleProgram
       ExampleSemantics ExampleIrisBase.
     Include IrisAdequacy DefaultBase ExampleSig ExampleProgram ExampleSemantics
-      ExampleIrisBase.
+      ExampleIrisBase ExampleIrisAdeqParams.
     Include ProgramLogicOn DefaultBase ExampleSig ExampleProgram ExampleSpecification.
     Include IrisInstanceWithContracts DefaultBase ExampleSig ExampleProgram
-      ExampleSemantics ExampleSpecification ExampleIrisBase.
+      ExampleSemantics ExampleSpecification ExampleIrisBase ExampleIrisAdeqParams.
 
     (* Verification of the absent foreign functions. *)
     Lemma foreignSem `{sailGS Σ} : ForeignSem.
